feat: finished proof of Lemma2
tockCSP_Network modified to distinguish refusals predicates from states.
TSF_Blocked definition of UngrantedNonTockRequest was modified to remove Tock from internal events and isBlockedInNonTock modified to use the whole Vocabulary instead of removing {tock}.

Lemma2 and Theorem1 now use NonTockBusyNetwork instead of BusyNetwork

TSF/TSF_Blocked.thy
@@ -16,24 +16,27 @@ where
 
 subsection \<open> Requests \<close>
 
-
 definition isUngrantedNonTockRequestOf :: "('i,'e) NetworkF => 'i => ('i,'e::tockCSP) net_state => 'i => bool"
       ("(1_ >> /(0_ (1/--tock[_]-->o) /_))" [800, 800,0,800] 900)
 where
-    "VF >> i --tock[sigma]-->o j == VF >> i --[sigma]--> j & ~ (sigma isTimeStopStateOf VF) &
+    "VF >> i --tock[sigma]-->o j ==
+        VF >> i --[sigma]--> j &
+        ~ (sigma isTimeStopStateOf VF) &
         Ev ` (snd (snd VF i)) Int Ev ` (snd (snd VF j)) - {Tock}
         <= (snd sigma) i Un (snd sigma) j"
+
 
 definition isUngrantedNonTockRequestOfwrt :: "('i,'e) NetworkF => 'i => ('i,'e) net_state => 'e::tockCSP set => 'i => bool"
       ("(1_ >> /(0_ (1/--tock[(0_,/_)]-->o) /_))" [800, 800,0,0,800] 900)
 where
-    "VF >> i --tock[sigma,Lambda]-->o j == VF >> i --tock[sigma]-->o j &
-        ((Ev ` (snd (snd VF i))) - (snd sigma) i) Un
-        ((Ev ` (snd (snd VF j))) - (snd sigma) j) <= Ev ` Lambda"
+    "VF >> i --tock[sigma,Lambda]-->o j ==
+        VF >> i --tock[sigma]-->o j &
+        (((Ev ` (snd (snd VF i))) - (snd sigma) i) Un
+         ((Ev ` (snd (snd VF j))) - (snd sigma) j)) - {Tock} <= Ev ` Lambda"
 
 
 
-subsection \<open> BlockedIn \<close>
+subsection \<open> BlockedIn NonTock \<close>
 
 
 definition  isBlockedInNonTock :: "('i,'e) NetworkF => 'i => ('i,'e::tockCSP) net_state => bool"
@@ -43,15 +46,26 @@ where
           tock_triple_conjoint VF &
           (EX j. VF >> i --[sigma]--> j) &
           (ALL j. VF >> i --[sigma]--> j
-          --> (VF >> i --tock[sigma, (VocabularyOf VF) - {tock}]-->o j))"
+          --> (VF >> i --tock[sigma, (VocabularyOf VF)]-->o j))"
 
 
 
 
-subsection \<open> Auxiliary lemmas \<close>
+
+subsection \<open> Lemmas \<close>
+
+subsubsection \<open> tock_triple_conjoint \<close>
 
 
-subsubsection \<open> Auxiliary lemmas - in index I \<close>
+lemma tock_triple_conjoint_PXf_FXf :
+    "tock_triple_conjoint (I,PXf) \<Longrightarrow> (I,FXf) isFailureOf (I,PXf) \<Longrightarrow>
+     tock_triple_conjoint (I,FXf)"
+  apply (simp add: tock_triple_conjoint_def)
+  by (simp add: isFailureOf_def)
+
+
+
+subsubsection \<open> ungranted requests --> in index I \<close>
 
 lemma in_index_NonTock_I1:
   "(I, FXf) >> i --tock[sigma]-->o j ==> i : I & j : I & i ~= j"
@@ -69,7 +83,9 @@ lemmas in_index_NonTock_I = in_index_NonTock_I1 in_index_NonTock_I2
 
 
 
-subsubsection \<open> Auxiliary lemmas - sub request \<close>
+
+
+subsubsection \<open> ungranted requests --> subset \<close>
 
 lemma isUngrantedNonTockRequestOf_subsetI:
   "[| (I, FXf) >> i --tock[(t,Yf)]-->o j; J <= I; i:J ; j:J ; 
@@ -78,12 +94,13 @@ lemma isUngrantedNonTockRequestOf_subsetI:
 apply (simp add: isUngrantedNonTockRequestOf_def)
 apply (rule)
 apply (rule isRequestOf_subsetI, simp_all)
-apply (simp add: isTimeStopStateOf_def, elim conjE)
+apply (simp add: isTimeStopStateOf_def refusesTock_def, elim conjE)
 apply (rule)
 apply (simp add: isRequestOf_def, elim conjE)
 apply (rule)
 apply (drule_tac x=x in spec, fast)
 done
+
 
 lemma isUngrantedNonTockRequestOfwrt_subsetI:
   "[| (I, FXf) >> i --tock[(t,Yf), Lambda1]-->o j; J <= I; i:J ; j:J ; 
@@ -97,210 +114,70 @@ apply (blast)
 done
 
 
+subsubsection \<open> requests intro \<close>
 
-subsubsection \<open> Auxiliary lemmas - is________StateOf \<close>
-
-lemma isDeadlockStateOf_if_isNonTockDeadlockStateOf :
-    "(t, Yf) isNonTockDeadlockStateOf (I, FXf) \<Longrightarrow>
-    (t, Yf) isDeadlockStateOf (I, FXf)"
-  by (simp add: isNonTockDeadlockStateOf_def)
-(*  by (simp add: isDeadlockStateOf_def) *)
-
-
-lemma BusyNetwork_if_NonTockBusyNetwork :
-    "NonTockBusyNetwork (I, FXf) \<Longrightarrow> BusyNetwork (I, FXf)"
-  by (simp add: NonTockBusyNetwork_def)
-
-
-
-lemma not_isTimeStopStateOf_if_isNonTockDeadlockStateOf :
-    "sigma isNonTockDeadlockStateOf VF \<Longrightarrow>
-    ~ (sigma isTimeStopStateOf VF)"
-  by (simp add: isNonTockDeadlockStateOf_def)
-
-
-
-lemma Tock_notin_refusals_if_not_isTimeStopStateOf :
-    "~ (sigma isTimeStopStateOf VF) \<Longrightarrow> sigma isStateOf VF \<Longrightarrow>
-    Tock \<notin> Union {((snd sigma) i) |i. i : fst VF}"
-  by (simp add: isTimeStopStateOf_def)
-
-
-lemma Tock_notin_refusals_if_isNonTockDeadlockStateOf :
-    "sigma isNonTockDeadlockStateOf VF \<Longrightarrow>
-    Tock \<notin> Union {((snd sigma) i) |i. i : fst VF}"
-  apply (simp only: isNonTockDeadlockStateOf_def)
-  apply (simp only: isDeadlockStateOf_def, elim conjE)
-  by (simp add: isTimeStopStateOf_def)
-
-
-
-lemma refusals_are_subsets_if_isStateOf :
-    "(t,Yf) isStateOf (I,FXf) \<Longrightarrow>
-     ALL i:I. Yf i <= (Ev ` (snd (FXf i)))"
-  apply (simp add: isStateOf_def)
-  done
-
-lemma refusals_are_subsets_if_isDeadlockStateOf :
-    "(t,Yf) isDeadlockStateOf (I,FXf) \<Longrightarrow>
-     ALL i:I. Yf i <= (Ev ` (snd (FXf i)))"
-  apply (simp only: isDeadlockStateOf_def, elim conjE)
-  apply (rule refusals_are_subsets_if_isStateOf, simp)
-  done
-
-lemma refusals_are_subsets_if_isNonTockDeadlockStateOf :
-    "(t,Yf) isNonTockDeadlockStateOf (I,FXf) \<Longrightarrow>
-     ALL i:I. Yf i <= (Ev ` (snd (FXf i)))"
-  apply (simp only: isNonTockDeadlockStateOf_def, elim conjE)
-  apply (rule refusals_are_subsets_if_isDeadlockStateOf, simp)
-  done
-                             
-
-lemma in_refusals_if_isDeadlockStateOf :
-    "(t, Yf) isDeadlockStateOf (I, FXf) \<Longrightarrow>
-     i \<in> I \<Longrightarrow> j \<in> I \<Longrightarrow> i \<noteq> j \<Longrightarrow>
-     x \<in> Ev ` snd (FXf i) \<inter> Ev ` snd (FXf j) \<Longrightarrow>
-     x : Union {Yf i |i. i : I}"
-  apply (simp add: isDeadlockStateOf_def)
-
-  apply (simp add: isStateOf_def)
-  apply (simp add: ALP_def)
-  apply (simp add: image_iff)
-  apply (elim conjE bexE, simp)
-  
-  apply (rule_tac x="i" in bexI)
-  apply (simp, simp)
-  done
-
-lemma in_refusals_if_isNonTockDeadlockStateOf :
-    "(t, Yf) isNonTockDeadlockStateOf (I, FXf) \<Longrightarrow>
-     i \<in> I \<Longrightarrow> j \<in> I \<Longrightarrow> i \<noteq> j \<Longrightarrow>
-     x \<in> Ev ` snd (FXf i) \<inter> Ev ` snd (FXf j) - {Tock} \<Longrightarrow>
-     x : Union {Yf i |i. i : I}"
-  apply (frule isDeadlockStateOf_if_isNonTockDeadlockStateOf)
-  apply (drule in_refusals_if_isDeadlockStateOf, simp_all)
-  by (simp)
-
-
-
-lemma ex_Request_if_isDeadlockStateOf_BusyNetwork :
-    "(t, Yf) isDeadlockStateOf (I, FXf) \<Longrightarrow>
-     i \<in> I \<Longrightarrow> BusyNetwork (I, FXf) \<Longrightarrow>
+lemma ex_target_for_NonTockRequest_nonTock_refusals :
+    "(t, Yf) isNonTockDeadlockStateOf (I, FXf) ==>
+     i : I ==> Yf i ~= Ev ` snd (FXf i) - {Tock} ==>
      EX j. (I, FXf) >> i --[(t, Yf)]--> j"
+  apply (simp only: isRequestOf_def)
 
-  (* busy --> i is deadlock-free *)
-  apply (simp only: BusyNetwork_def)
-  apply (drule_tac x="i" in bspec, simp)
+  apply (frule isStateOf_if_isNonTockDeadlockStateOf)
+  apply (frule refusals_are_subsets_if_isStateOf)
 
-  (* Refusals are subsets *)
-  apply (frule refusals_are_subsets_if_isDeadlockStateOf)
+  apply (frule Union_refusals_ALP_if_isNonTockDeadlockStateOf)
+  apply (simp only: ALP_def)
 
-  apply (simp add: isRequestOf_def)
-  apply (simp add: isDeadlockStateOf_def)
-
-    (* EX j *)
-    apply (elim conjE)
-
-    (* Refusals i *)
-    apply (frule_tac x="i" in bspec, simp)
-  
-    apply (drule_tac x="t rest-tr (snd (FXf i))" in spec)
-    apply (drule_tac x="Yf" in spec)
-    apply (drule mp)
-    apply (rule isStateOf_each_element, simp, simp)
-    apply (simp add: ALP_def)
-
-    apply (subgoal_tac "EX a: Ev ` snd (FXf i). a ~: Yf i")        (* ... sub 1 *)
+  (* i is not refusing event a from its synchronisation set *)
+  apply (frule ex_non_refused_nonTock_event_if_isNonTockDeadlockStateOf[of t Yf I FXf i])
+    apply (simp_all)
     apply (elim bexE)
-    apply (subgoal_tac "a : Ev ` {a. EX i:I. a : snd (FXf i)}")    (* ... sub 2 *)
-      apply (rotate_tac 5)
-      apply (drule sym)
-      apply (simp)
-      apply (elim conjE exE)
-      apply (simp)
-      apply (rule_tac x="ia" in exI)
-      apply (case_tac "i = ia", simp)
-      apply (simp)
-      apply (drule_tac x="ia" in bspec, simp)
-      apply (simp only: Int_commute Int_Diff[THEN sym])
-      apply (rule)
-      apply (fast)
+  apply (subgoal_tac "Ev a : Ev ` {a. EX i:I. a : snd (FXf i)} - {Tock}")
+                                                  (* ... sub 1 *)
+  apply (rotate_tac 1)
+  apply (drule sym)
+  apply (simp)
+  apply (elim conjE exE)
+  apply (simp)
 
-     (* sub 2 *)
-     apply (blast)
-    (* sub 1 *)
-    apply (blast)
-  done
+  apply (rule_tac x="ia" in exI)
+  apply (case_tac "i = ia", simp)
+  apply (simp)
+  apply (drule_tac x="ia" in bspec, simp)
+  apply (fast)
 
-
-lemma ex_Request_if_isNonTockDeadlockStateOf_NonTockBusyNetwork :
-    "(t, Yf) isNonTockDeadlockStateOf (I, FXf) \<Longrightarrow>
-     i \<in> I \<Longrightarrow> NonTockBusyNetwork (I, FXf) \<Longrightarrow>
-     \<exists>j. (I, FXf) >> i --[(t, Yf)]--> j"
-  apply (frule isDeadlockStateOf_if_isNonTockDeadlockStateOf)
-  apply (frule BusyNetwork_if_NonTockBusyNetwork)
-  apply (rule ex_Request_if_isDeadlockStateOf_BusyNetwork, simp_all)
+  (* sub 1 *)
+  apply (blast)
   done
 
 
 
-lemma tock_notin_refusals_if_isNonTockDeadlockStateOf :
-    "(t, Yf) isNonTockDeadlockStateOf (I, FXf) \<Longrightarrow>
-       x \<in> \<Union> {Yf i |i. i \<in> I} \<Longrightarrow> x \<noteq> Tock"
-  apply (frule Tock_notin_refusals_if_isNonTockDeadlockStateOf)
-  by (force)
 
+lemma ex_NonTockRequest_if_isNonTockDeadlockStateOf_NonTockBusyNetwork :
+    "(t, Yf) isNonTockDeadlockStateOf (I, FXf) ==>
+     NonTockBusyNetwork (I, FXf) ==> 
+     i : I ==> ~ Ev ` snd (FXf i) <= {Tock} ==>
+     EX j. (I, FXf) >> i --[(t, Yf)]--> j"
+  apply (frule isStateOf_if_isNonTockDeadlockStateOf)
 
-lemma tock_notin_refusals_if_isNonTockDeadlockStateOf2 :
-    "(t, Yf) isNonTockDeadlockStateOf (I, FXf) \<Longrightarrow>
-       Ev x \<in> Yf i \<Longrightarrow> i \<in> I \<Longrightarrow> x \<noteq> tock"
-  apply (frule Tock_notin_refusals_if_isNonTockDeadlockStateOf)
-  by (force)
+  apply (rule ex_target_for_NonTockRequest_nonTock_refusals, simp_all)
 
+  (* refusing ALL events *)
+  apply (frule Union_refusals_ALP_if_isNonTockDeadlockStateOf, simp add: ALP_def)
 
+  (* NonTock busy --> i is time-stop-free *)
+  apply (simp only: NonTockBusyNetwork_def)
 
+  (* State of i *)
+  apply (drule_tac x="i" in bspec, simp)
+  apply (drule_tac x="(t rest-tr (snd (FXf i)), Yf)" in spec)
 
+  apply (simp add: isNonTockDeadlockStateOf_def)
+  apply (drule mp, simp add: isStateOf_each_element)
 
-
-
-lemma hide_tr_Compl_isStateOf_subset: 
-  "[| (t,Yf) isStateOf (I,FXf) ; J <= I ; 
-      X = {sY. EX i:J. sY : snd (FXf i)} |]
-  ==> (t --tr (- X), Yf) isStateOf (J, FXf)"
-apply (simp add: isStateOf_def ALP_def)
-apply (rule conjI)
-apply (insert rest_tr_subset_event[of t "X"])
-apply (subgoal_tac "Tick ~: sett (t --tr (- X))")
-apply (force)
-apply (force)
-
-apply (rule ballI)
-apply (elim conjE)
-apply (drule_tac x="i" in bspec, fast)
-
-apply (simp add: rest_tr_def)
-
-apply (subgoal_tac "snd (FXf i) <= {sY. EX i:J. sY : snd (FXf i)}")
-apply (simp add: hide_tr_of_hide_tr_subset)
-by (auto)
-
-
-lemma hide_tr_Compl_isStateOf_subsetI:
-  "[| (t,Yf) isStateOf (I,FXf) ; 
-      J <= I ; X = Union {(snd (FXf i))|i. i:J} |]
-  ==> (t --tr (- X), Yf) isStateOf (J, FXf)"
-apply (subgoal_tac "Union {(snd (FXf i))|i. i:J} = {sY. EX i:J. sY : snd (FXf i)}")
-apply (simp add: hide_tr_Compl_isStateOf_subset)
-by (auto)
-
-
-
-lemma tock_triple_conjoint_PXf_FXf :
-    "tock_triple_conjoint (I,PXf) \<Longrightarrow> (I,FXf) isFailureOf (I,PXf) \<Longrightarrow>
-     tock_triple_conjoint (I,FXf)"
-  apply (simp add: tock_triple_conjoint_def)
-  by (simp add: isFailureOf_def)
-
+  apply (simp only: refusesAllNonTock_def refusesNonTock_def)
+  apply (simp add: ALP_def)
+  done
 
 
 
