TSF/TSF_Infra.thy
@@ -5,7 +5,7 @@ begin
 
 
 lemma insert_Tick_Evset_Un [simp]:
-    "insert Tick (Evset \<union> X) = EvsetTick"
+    "insert Tick (Evset Un X) = EvsetTick"
   apply (simp only: insert_def Un_left_commute)
   by (subst Evset_Un_eq_EvsetTick_if, simp_all)
 
@@ -94,81 +94,6 @@ lemma Tick_notin_src_tocks_nontocks_nilt_iff :
 
 
 
-(*
-lemma tocks_neq_nontocks :
-    "t ~= <> \<and> t ~= <Tick> \<Longrightarrow>
-     t =nontocks(s) = t \<noteq>tocks(s)"
-  apply (elim conjE, rule)
-  apply (drule nontocks_only_if, simp)
 
-  apply (induct s rule: induct_trace)
-  apply (simp)
-  by (case_tac "a = tock", simp, simp)
-
-
-  apply (rotate_tac 2)
-  apply (induct t rule: induct_trace, simp_all)
-  apply (drule hide_tr_decompo_neq_Ev_appt_only_if)
-  apply (simp)
-defer
-  apply (drule hide_tr_Compl_singleton_only_if)
-*)
-
-
-
-(*
-declare [[show_types]]
-declare [[show_sorts]]
-(*     | (\<forall>tnt. \<exists> t nt. \<exists> merge::'e trace \<Rightarrow> 'e trace \<Rightarrow> 'e::tockCSP trace.
-                      tnt = merge t nt &
-                      t :t traces (P -- Nontock) MT &
-                      nt :t traces (P -- {tock}) MT &
-                      (tnt,X) ~:f failures P MF)*)
-lemma merge_tock_nontock :
-    "(\<forall>tnt. \<exists> t nt. \<exists> merge::'e trace \<Rightarrow> 'e trace \<Rightarrow> 'e::tockCSP trace.
-                          tnt = merge t nt &
-                          t :t traces (P -- Nontock) MT &
-                          nt :t traces (P -- {tock}) MT &
-                          (tnt,X) :f failures P MF)"
-  apply (rule, simp_all add: in_traces)
-  oops
-*)
-
-
-(*
-
-lemma hide_tr_non_x_sett_if :
-    "(sett s <= {Tick,Ev x}) \<and> (t ~= <> \<and> t ~= <Tick>) \<Longrightarrow> (t --tr (- {x}) = s)"
-  apply (simp add: subset_doubleton_iff)
-  apply (elim conjE disjE)
-  apply (simp_all add: sett_empty_iff sett_Tick_iff)
-    apply (simp add: hide_tr_non_x_sett)
-
-  apply (induct t arbitrary: x rule: induct_trace)
-    apply (simp_all)
-    apply (simp, drule sym, simp)
-    apply (simp_all)
-    apply (drule sym, simp)
-  done
-
-lemma nontocks_if :
-    "t \<noteq>tocks(s) \<Longrightarrow> t =nontocks(s)"
-  apply (erule contrapos_np)
-    apply (subst hide_tr_non_x_sett)
-  oops
-
-lemma neq_hide_tr_single_if :
-    "(s --tr {x} ~= t) \<Longrightarrow> (s --tr (- {x}) = t) \<and> t ~= <> \<and> t ~= <Tick>"
-  apply (rule)
-  apply (subst hide_tr_cases_iff)
-  apply (rule, rule, simp)
-    apply (erule contrapos_np)
-    apply (subst hide_tr_nilt_sett)
-  apply (simp add: subset_doubleton_iff)
-  apply (elim disjE, simp_all)
-  apply (simp add: sett_empty_iff)
-  apply (simp add: sett_Tick_iff)
-  done
-*)
 
 end
