TSF/TSF_Lemma2.thy
@@ -7,250 +7,205 @@ subsection \<open> Lemma 2 \<close>
 
 
 (*** only if ***)
+
 lemma Lemma2_Jesus_Sampaio_2022_only_if:
-    "[| tock_triple_conjoint (I,FXf) ; BusyNetwork (I,FXf) ;
-        (t,Yf) isNonTockDeadlockStateOf (I,FXf) |]
+    "[| tock_triple_conjoint (I,FXf) ; NonTockBusyNetwork (I,FXf) ;
+        (t,Yf) isNonTockDeadlockStateOf (I,FXf) ;
+        ALL i:I. ~ Ev ` snd (FXf i) <= {Tock} |]
      ==> ALL i:I. (I,FXf) >> i isBlockedInNonTock (t,Yf)"
   (* ALL i *)
   apply (intro ballI)
 
   (* Refusals are subsets *)
-  apply (frule refusals_are_subsets_if_isNonTockDeadlockStateOf)
+  apply (frule isStateOf_if_isNonTockDeadlockStateOf)
+  apply (frule refusals_are_subsets_if_isStateOf, simp)
+  apply (frule refusals_are_subsetsNonTock_if_isNonTockDeadlockStateOf)
 
   apply (simp only: isBlockedInNonTock_def)
     (* tock_triple_conjoint AND ... *)
     apply (rule conjI, simp)
-    (* EX nonTockRequest AND
-       ALL nontockRequest IMPLIES ungratedNonTockRequest *)
+    (* EX request AND
+       ALL request IMPLIES ungratedNonTockRequest *)
     apply (rule conjI)
 
-  (* EX nonTockRequest FROM i TO j *)
-    apply (frule isDeadlockStateOf_if_isNonTockDeadlockStateOf)
-    apply (rule ex_Request_if_isDeadlockStateOf_BusyNetwork, simp_all)
+    (* EX nonTockRequest FROM i TO j *)
+    apply (rule ex_NonTockRequest_if_isNonTockDeadlockStateOf_NonTockBusyNetwork, simp_all)
 
-  (* ALL j *)
+    (* ALL j *)
     apply (intro allI impI)
 
-    (* ALL nontockRequest FROM i TO j IMPLIES ungratedNonTockRequest FROM i TO j *)
+    (* ALL request FROM i TO j ARE Ungrated NonTock Requests *)
     apply (unfold isUngrantedNonTockRequestOfwrt_def)
 
     apply (rule conjI)
-      apply (simp add: isUngrantedNonTockRequestOf_def)
-      apply (frule not_isTimeStopStateOf_if_isNonTockDeadlockStateOf, simp)
 
-      (* Request FROM i TO j *)
-      apply (simp add: isRequestOf_def)
+    (* 1-2 *)
+    apply (simp add: isUngrantedNonTockRequestOf_def)
+    apply (frule not_isTimeStopStateOf_if_isNonTockDeadlockStateOf, simp)
 
-      (* alpha i INT alpha j SUBSET Un refusals *)
-      apply (rule)
-      (* x is a refusal *)
-      (* "Creates" the third index ia *)
-      apply (subgoal_tac "x : Union {Yf i |i. i : I}")
+    (* Request FROM i TO j *)
+    apply (simp add: isRequestOf_def)
 
-       apply (simp)
-       apply (elim conjE bexE exE)
-       apply (case_tac "ia = i", simp)
-       apply (case_tac "ia = j", simp)
-       (* ia ~= i & ia ~= j ==> contradict with tock_triple_conjoint *)
-       apply (drule_tac x="ia" in bspec, simp)
-       apply (simp add: isDeadlockStateOf_def isStateOf_def)
-       apply (simp add: tock_triple_conjoint_def)
-       apply (drule_tac x="i" in bspec, simp)
-       apply (drule_tac x="j" in bspec, simp)
-       apply (drule_tac x="ia" in bspec, simp)
-        apply (drule mp)
-        apply (simp)
-       apply (rotate_tac 5)
-       apply (erule contrapos_pp)
-       apply (blast)
+    (* alpha i INT alpha j SUBSET Un refusals *)
+    apply (rule)
+    (* x is a refusal *)
 
-       apply (rule_tac i=i and j=j in in_refusals_if_isNonTockDeadlockStateOf[of t Yf I FXf])
-         apply (simp, simp, simp, simp, simp)
+    (* "Creates" the third index ia *)
+    apply (subgoal_tac "x : (netRefusals I Yf)")
+
+     apply (simp)
+     apply (elim conjE bexE exE)
+     apply (case_tac "ia = i", simp)
+     apply (case_tac "ia = j", simp)
+     (* ia ~= i & ia ~= j ==> contradict with tock_triple_conjoint *)
+     apply (simp add: tock_triple_conjoint_def)
+     apply (blast)
+
+     apply (rule_tac i=i and j=j in in_refusals_if_isNonTockDeadlockStateOf[of t Yf I FXf])
+       apply (simp, simp, simp, simp, simp)
 
      (* 2-2 *)
-      apply (rule)
-      apply (simp only: VocabularyOf_def)
-      apply (subgoal_tac "x : Union {Yf i |i. i : I}")
+     apply (rule)
+     apply (simp only: VocabularyOf_def)
+     apply (subgoal_tac "x : netRefusals I Yf")
 
-       apply (simp)
-       apply (elim conjE bexE exE)
-       apply (simp add: image_iff)
-       apply (elim disjE conjE bexE)
+     apply (simp)
+     apply (elim conjE bexE exE)
+     apply (simp add: image_iff)
+     apply (elim disjE conjE bexE)
 
-        apply (case_tac "i = ia", simp)
-        apply (drule_tac x="ia" in bspec, simp)
-        apply (simp add: isStateOf_def)
-        apply (rule)
-        apply (rule_tac x="(snd (FXf i) Int snd (FXf ia))" in exI)
-        apply (rule conjI)
-         apply (rule_tac x="i" in bexI)
-         apply (rule_tac x="ia" in bexI)
-         apply (simp)
-         apply (simp)
-         apply (simp)
-         apply (blast)
+      apply (case_tac "i = ia", simp)
+      apply (drule_tac x="ia" in bspec, simp)
+      apply (simp add: isStateOf_def)
+        apply (rule_tac x="(snd (FXf i) Int snd (FXf ia))" in exI, blast)
 
-        apply (rule tock_notin_refusals_if_isNonTockDeadlockStateOf2, simp, simp, simp)
+      apply (case_tac "j = ia", simp)
+      apply (drule_tac x="ia" in bspec, simp)
+      apply (simp only: isRequestOf_def, elim conjE)
+      apply (simp add: isStateOf_def)
+        apply (rule_tac x="snd (FXf j) Int snd (FXf ia)" in exI, blast)
 
-        apply (case_tac "j = ia", simp)
-        apply (drule_tac x="ia" in bspec, simp)
-        apply (simp only: isRequestOf_def, elim conjE)
-        apply (simp add: isStateOf_def)
-        apply (rule)
-        apply (rule_tac x="snd (FXf j) Int snd (FXf ia)" in exI)
-        apply (rule conjI)
-         apply (rule_tac x="j" in bexI)
-         apply (rule_tac x="ia" in bexI)
-         apply (simp)
-         apply (simp)
-         apply (simp add: isRequestOf_def)
-         apply (blast)
-
-        apply (rule tock_notin_refusals_if_isNonTockDeadlockStateOf2, simp, simp, simp)
-
-  apply (simp only: Un_iff isNonTockDeadlockStateOf_def)
-  apply (simp only: isDeadlockStateOf_def)
-  apply (simp add: isDeadlockStateOf_def)
-  apply (simp add: ALP_def)
-
-  apply (simp add: image_iff)
-  apply (elim disjE conjE bexE)
-
-   apply (rule_tac x="xa" in exI)
-   apply (simp)
-   apply (fast)
-
-   apply (rule_tac x="xa" in exI)
-   apply (simp)
-   apply (rule_tac x="j" in bexI)
-   apply (simp)
-   apply (simp add: isRequestOf_def)
+      apply (simp only: isRequestOf_def)
+      apply (simp add: isNonTockDeadlockStateOf_def)
+      apply (simp add: refusesAllNonTock_def refusesNonTock_def)
+      apply (simp add: subset_singleton_iff)
+      apply (simp add: Diff_eq Int_def ALP_def)
+      apply (elim conjE)
+      apply (simp only: Union_eq set_eq_iff)
+      apply (drule_tac x="x" in spec, simp)
+      apply (erule disjE, fast, fast)
   done
 
 
 
 (*** if ***)
 
+
+
+(* ALL synchronisation sets are Tock \<union> X where X \<noteq> {} *)
 lemma Lemma2_Jesus_Sampaio_2022_if:
-    "[| tock_triple_conjoint (I,FXf) ; BusyNetwork (I,FXf) ;
-        (t,Yf) isStateOf (I,FXf) ;
-        ALL i:I. (I,FXf) >> i isBlockedInNonTock (t,Yf) |]
+    "[| tock_triple_conjoint (I,FXf) ; NonTockBusyNetwork (I,FXf) ;
+        (t, Yf) isStateOf (I, FXf) ; 
+        ALL i:I. (I,FXf) >> i isBlockedInNonTock (t,Yf) ;
+        ALL i:I. ~ Ev ` snd (FXf i) <= {Tock} |]
      ==> (t,Yf) isNonTockDeadlockStateOf (I,FXf)"
+
   apply (simp add: isNonTockDeadlockStateOf_def)
-  apply (rule)
-  apply (simp add: isDeadlockStateOf_def)
-  apply (simp add: ALP_def)
-  apply (rule)
-  
-   (* <= *)
-   apply (rule)
-   apply (simp)
-   apply (elim exE conjE)
-   apply (simp)
-   apply (drule_tac x="i" in bspec, simp)
-   apply (simp add: isStateOf_def)
-   apply (elim conjE)
-   apply (drule_tac x="i" in bspec, simp)
-   apply (simp add: ALP_def)
-   apply (force)
+  apply (simp add: refusesAllNonTock_def)
 
-   (* => *)
-   apply (rule)
-   apply (simp)
-   apply (simp only: isBlockedInNonTock_def)
-   apply (simp add: image_iff)
-   apply (elim conjE exE bexE)
-   apply (simp)
-   
-   apply (case_tac "Ev xa : Yf i")
+  apply (rule)
+
+  (* <= *) (* netRefusals <= ALP - {Tock} *)
+  (*apply (insert ex_in_conv[of I], simp, elim exE)
+  apply (rename_tac i)*)
+  apply (rule)
+  apply (rule)
+    apply (simp add: isStateOf_def ALP_def, elim conjE, fast)
+    apply (simp)
+    apply (elim exE conjE)
+    apply (simp)
+    apply (drule_tac x="i" in bspec, simp)
+    apply (drule_tac x="i" in bspec, simp only:)
+    apply (simp only: isBlockedInNonTock_def, elim conjE exE)
+    apply (drule_tac x=j in spec, simp)
+    apply (simp add: isUngrantedNonTockRequestOfwrt_def)
+    apply (simp add: isUngrantedNonTockRequestOf_def)
+    apply (simp add: isTimeStopStateOf_def refusesTock_def)
+    apply (simp add: isStateOf_def ALP_def, elim conjE, blast)
+
+  (* => *) (* ALP - {Tock} <= netRefusals *)
+  apply (rule)
+  apply (simp)
+  (* an event x (~= Tock) from the net ALP is being refused *)
+  apply (simp only: isBlockedInNonTock_def)
+    apply (simp only: image_iff ALP_def)
+    apply (elim conjE exE bexE)
+    apply (drule CollectD)
+    apply (elim bexE)
+    apply (rename_tac e ev i)
+  
+    apply (case_tac "Ev ev : Yf i")
     apply (rule_tac x="Yf i" in exI)
+    apply (simp, fast)
+
+    (* Ev ev ~: Yf i *)
+    apply (subgoal_tac "ev : VocabularyOf (I,FXf) - {tock}")
+
+    apply (simp add: VocabularyOf_def)
+    apply (elim conjE exE bexE)
+    apply (simp)
+    
+    apply (case_tac "ia = i")
+    apply (simp)
+    apply (drule_tac x="i" in bspec, simp)
+    apply (elim conjE exE)
+
+    apply (drule_tac x="j" in spec)
+    apply (drule mp)
+    apply (simp add: isRequestOf_def)
+    apply (blast)
+
+    apply (simp add: isUngrantedNonTockRequestOfwrt_def)
+    apply (simp add: isUngrantedNonTockRequestOf_def)
+    apply (rule_tac x="Yf j" in exI)
     apply (fast)
-  
-   (* Ev xa ~: Yf i *)
-    apply (subgoal_tac "xa : VocabularyOf (I,FXf) - {tock}")
-     apply (simp add: VocabularyOf_def)
-     apply (elim conjE exE bexE)
-     apply (simp)
-  
-     apply (case_tac "ia = i")
-      apply (simp)
-      apply (drule_tac x="i" in bspec, simp)
-      apply (elim conjE exE)
-  
-      apply (drule_tac x="j" in spec)
-      apply (drule mp)
-      apply (simp add: isRequestOf_def)
-      apply (blast)
-  
-      apply (simp add: isUngrantedNonTockRequestOfwrt_def)
-      apply (simp add: isUngrantedNonTockRequestOf_def)
-      apply (simp only: isTimeStopStateOf_def de_Morgan_conj)
-      apply (rule_tac x="Yf j" in exI)
-      apply (fast)
 
-     apply (case_tac "j = i")
-      apply (simp)
-      apply (drule_tac x="i" in bspec, simp)
-      apply (elim conjE exE)
-       apply (drule_tac x="ia" in spec)
-       apply (drule mp)
-       apply (simp add: isRequestOf_def)
-       apply (blast)
-  
-       apply (simp add: isUngrantedNonTockRequestOfwrt_def)
-       apply (simp add: isUngrantedNonTockRequestOf_def)
-       apply (simp only: isTimeStopStateOf_def de_Morgan_conj)
-       apply (rule_tac x="Yf ia" in exI)
-       apply (fast)
-  
-     (* ia ~= i; j ~= i; ia ~= j, but xa : snd (PXf i), ... *)
-     apply (simp add: tock_triple_conjoint_def)
-     apply (drule_tac x="i" in bspec, simp)
-     apply (rotate_tac -1)
-     apply (drule_tac x="ia" in bspec, simp)
-     apply (rotate_tac -1)
-     apply (drule_tac x="j" in bspec, simp)
-     apply (fast)
+   apply (case_tac "j = i")
+    apply (simp)
+    apply (drule_tac x="i" in bspec, simp)
+    apply (elim conjE exE)
+     apply (drule_tac x="ia" in spec)
+     apply (drule mp)
+     apply (simp add: isRequestOf_def)
+     apply (blast)
 
-
-    (* xa : VocabularyOf VF - {tock} *)
-     apply (simp, rule)
-
-     apply (drule_tac x="i" in bspec, simp)
-     apply (elim exE conjE)
-     apply (drule_tac x="xb" in spec)
      apply (simp add: isUngrantedNonTockRequestOfwrt_def)
      apply (simp add: isUngrantedNonTockRequestOf_def)
+     apply (rule_tac x="Yf ia" in exI)
      apply (fast)
 
-     apply (drule_tac x="i" in bspec, simp)
-     apply (elim exE conjE)
-     apply (drule_tac x="xb" in spec, simp)
-     apply (simp add: isUngrantedNonTockRequestOfwrt_def)
-     apply (simp add: isUngrantedNonTockRequestOf_def)
-     apply (elim conjE)
-     apply (frule Tock_notin_refusals_if_not_isTimeStopStateOf, simp)
+    (* ia ~= i; j ~= i; ia ~= j, but xa : snd (PXf i), ... *)
+    apply (simp add: tock_triple_conjoint_def)
+    apply (drule_tac x="i" in bspec, simp)
+    apply (rotate_tac -1)
+    apply (drule_tac x="ia" in bspec, simp)
+    apply (rotate_tac -1)
+    apply (drule_tac x="j" in bspec, simp)
+    apply (fast)
 
-       apply (simp add: VocabularyOf_def)
-       apply (simp only: isRequestOf_def, elim conjE)
-       apply (drule_tac x="Yf xb" in spec)
-       apply (erule disjE, simp, simp)
-       apply (simp add: subset_iff)
-       apply (fast)
-
-    (* ~ isTimeStopStateOf *)
-       apply (simp only: isBlockedInNonTock_def)
-       apply (simp add: isUngrantedNonTockRequestOfwrt_def)
-       apply (simp add: isUngrantedNonTockRequestOf_def)
-       apply (simp only: isTimeStopStateOf_def de_Morgan_conj)
-       apply (rule disjI2, simp)
-       apply (fast)
-  done
+    apply (simp add: VocabularyOf_def)
+    apply (drule_tac x="i" in bspec, simp)
+    apply (elim exE conjE)
+    apply (drule_tac x="x" in spec)
+    apply (simp add: isUngrantedNonTockRequestOfwrt_def, elim conjE)
+    apply (blast)
+done
 
 
 lemma Lemma2_Jesus_Sampaio_2022:
-    "[| tock_triple_conjoint (I,FXf) ; BusyNetwork (I,FXf) ; 
-        (t,Yf) isStateOf (I,FXf) |]
+    "[| tock_triple_conjoint (I,FXf) ; NonTockBusyNetwork (I,FXf) ;
+        (t,Yf) isStateOf (I,FXf) ; 
+        ALL i:I. ~ Ev ` snd (FXf i) <= {Tock} |]
      ==> (t,Yf) isNonTockDeadlockStateOf (I,FXf)
          = (ALL i:I. (I,FXf) >> i isBlockedInNonTock (t,Yf))"
   apply (rule)
